BrokenDevice/Definitions.v
@@ -1,0 +1,106 @@
+Require Import Lia.
+Require Import Bool.
+Require Import List.
+Import PeanoNat.Nat.
+Import ListNotations.
+Require Extraction.
+Require Import Program.Wf.
+Require Import Arith.Wf_nat.
+
+Inductive bit := B1 | B0.
+
+Definition broken_list := list bool.
+Definition message := list bit.
+Definition packet : Set := bit * bit * bit.
+Definition chunk : Set := bool * bool * bool.
+
+
+Fixpoint bools_to_chunks (p : broken_list) : list chunk :=  match p with
+  | a :: b :: c :: rest => (a,b,c) :: bools_to_chunks rest
+  | _ => []
+  end.
+
+Definition sum_chunk '((a,b,c) : chunk) := b2n a + b2n b + b2n c.
+
+Fixpoint packets_to_message (ps : list packet) := match ps with
+  | [] => []
+  | (a,b,c) :: rest => a :: b :: c :: packets_to_message rest
+  end.
+
+Fixpoint message_to_packets (x : message) := match x with
+  | a :: b :: c :: rest => (a,b,c) :: message_to_packets rest
+  | _ => []
+  end.
+
+(** Converting a list of packets to a message and back to packets is the identity. *)
+Lemma packets_message_inverses : forall ps,
+  message_to_packets (packets_to_message ps) = ps.
+Proof.
+  intros.
+  induction ps as [| p ps IH].
+  - reflexivity.
+  - destruct p as [[a b] c]. simpl. rewrite IH. reflexivity.
+Qed.
+
+Definition encode_packet '((a,b,c) : chunk) (x : message) : packet := 
+    let '(b1, b2) := (match x with
+      | []                => (B0 , B0)
+      | [b1']             => (b1', B0)
+      | b1' :: b2' :: bs' => (b1', b2')
+    end) in
+    match sum_chunk (a,b,c) with
+    | 0 => (match b1, b2 with
+        | B0, B0 => (B0, B1, B1)
+        | B0, B1 => (B1, B1, B1)
+        | B1, B0 => (B1, B0, B0)
+        | B1, B1 => (B1, B0, B1)
+        end)
+    | 1 => if a then (match b1 with
+        | B0 => (B0, B0, B1)
+        | B1 => (B0, B1, B0)
+        end)
+        else if c then (match b1 with
+        | B0 => (B1, B1, B0)
+        | B1 => (B0, B1, B0)
+        end)
+        else (match b1, b2 with
+        | B0, _  => (B0, B0, B1)
+        | B1, B0 => (B1, B0, B0)
+        | B1, B1 => (B1, B0, B1)
+        end)
+    | _ => (B0, B0, B0)
+    end.
+
+Definition decode_packet (p : packet) : message := match p with
+    | (B0, B0, B0) => []
+    | (B0, B0, B1) => [B0]
+    | (B0, B1, B0) => [B1]
+    | (B0, B1, B1) => [B0; B0]
+    | (B1, B0, B0) => [B1; B0]
+    | (B1, B0, B1) => [B1; B1]
+    | (B1, B1, B0) => [B0]
+    | (B1, B1, B1) => [B0; B1]
+    end.
+
+Fixpoint drop {A} (n : nat) (l : list A) : list A := match n, l with
+  | 0  , l       => l
+  | n  , []      => l
+  | S n, x :: ls => drop n ls
+  end.
+
+Fixpoint encode (x : message) (p : list chunk) : list packet := match p with
+  | c :: rest => let pack := encode_packet c x in
+    pack :: encode (drop (length (decode_packet pack)) x) rest
+  | _ => []
+  end.
+
+Fixpoint decode (x : list packet) : message := match x with
+  | p :: rest => decode_packet p ++ decode rest
+  | _ => []
+  end.      
+
+Definition anna (x : message) (p : broken_list) : message :=
+  packets_to_message (encode x (bools_to_chunks p)).
+
+Definition bruno (x : message) : message :=
+  decode (message_to_packets x).
