BrokenDevice/EncodeNat.v
@@ -1,0 +1,120 @@
+Require Import Lia.
+Require Import Bool.
+Require Import List.
+Import PeanoNat.Nat.
+Import ListNotations.
+Require Extraction.
+Require Import Program.Wf.
+Require Import Arith.Wf_nat.
+
+Require Import Definitions.
+
+Fixpoint decode_nat (x : message) : nat := match x with
+  | [] => 0
+  | x :: xs => (if x then 1 else 0) + 2 * decode_nat xs
+  end.
+
+Fixpoint div2 (n acc : nat) : nat * bool := match n with
+  | 0       => (0,false)
+  | 1       => (0,true)
+  | S (S n) => div2 n (S acc)
+  end.
+
+Lemma div2_nk : forall n k,
+   fst (div2 n (S k)) <= S (fst (div2 n k)) /\
+   fst (div2 (S n) (S k)) <= S (fst (div2 (S n) k)).
+Proof.
+  induction n; intros.
+  simpl. lia.
+  split. destruct (IHn k). auto. 
+  simpl. destruct (IHn (S k)). lia.
+Qed.
+
+Lemma div2_le : forall n k, n <> 0 -> 
+  fst (div2 n k) < n + k /\
+  fst (div2 (S n) k) < S n + k.
+Proof.
+  intros.
+  generalize dependent k.
+  induction n; intros. exfalso; apply H; auto.
+  destruct n. simpl. lia.
+  simpl. specialize IHn with k. destruct IHn as [IH1 IH2]. auto.
+  split. change (div2 n (S k)) with (div2 (S (S n)) k). lia.
+  destruct n. simpl. lia.
+  simpl. change (div2 n (S (S k))) with (div2 (S (S n)) (S k)). 
+  pose proof (div2_nk (S (S n)) k). lia.
+Qed.
+
+Lemma div2_le_0 : forall n, n <> 0 ->
+  fst (div2 n 0) < n.
+Proof. intros. destruct (div2_le n 0); auto. lia.
+Qed.
+
+(*
+Definition encode_nat (n : nat) : message.
+Proof.
+  Check lt_wf_rec.
+  apply (lt_wf_rec). auto.
+  intros n' H.
+  destruct (div2 n' 0) eqn:?.
+  destruct n0, b eqn:?; simpl in *.
+  - (*0, true *) exact [B1].
+  - (*0, false *) exact [].
+  - assert (fst (div2 n' 0) = S n0). rewrite Heqp; auto. 
+    apply (cons B1). apply H with (S n0). rewrite <- H0. apply div2_le_0. destruct n'; discriminate.
+  - assert (fst (div2 n' 0) = S n0). rewrite Heqp; auto. 
+    apply (cons B0). apply H with (S n0). rewrite <- H0. apply div2_le_0. destruct n'; discriminate.
+Defined.
+Print encode_nat.
+*)
+
+Program Fixpoint encode_nat (n : nat) {measure n}: message := match div2 n 0 with
+  | (0, false) => []
+  | (0, true)  => [B1]
+  | (m, false) => B0 :: encode_nat m
+  | (m, true)  => B1 :: encode_nat m
+  end.
+Next Obligation.
+  destruct n. inversion Heq_anonymous. subst. unfold "<>" in H.
+  exfalso; apply H; auto.
+  pose proof (div2_le_0 (S n)). 
+  assert (fst (div2 (S n) 0) = m). rewrite <- Heq_anonymous. auto. lia.
+Defined.
+Next Obligation. 
+  destruct n. inversion Heq_anonymous. 
+  destruct (div2_le (S n) 0). auto.
+  assert (fst (div2 (S n) 0) = m). rewrite <- Heq_anonymous. auto. lia.
+Defined.
+
+(** Reduction lemma. Still don't know how to properly work with Program Fixpoints... *)
+
+Lemma encode_nat_recurse : forall n m b,
+  n > 1 ->
+  div2 n 0 = (m, b) ->
+  encode_nat n = match b with
+    | false => B0 :: encode_nat m
+    | true  => B1 :: encode_nat m
+  end.
+Proof.
+  intros.
+  unfold encode_nat; simpl. rewrite fix_sub_eq. simpl. fold encode_nat. remember (div2 n 0) as A. rewrite H0. 
+  destruct m. simpl. subst. admit.
+  Admitted.
+
+(** The main theorem relating encoding and decoding: encode_nat and decode_nat are inverses. This is the lemma that is needed for the final proof. *)
+Lemma encode_inv : forall X,
+  X = decode_nat (encode_nat X).
+Proof.
+  intros.
+  induction X using lt_wf_ind. 
+  destruct (div2 X 0) eqn:?. destruct X. auto. 
+  assert (n < S X). { assert (n = fst (div2 (S X) 0)). rewrite Heqp. auto. rewrite H0. apply div2_le_0; auto. }
+  specialize H with n.
+  pose proof (encode_nat_recurse (S X) n b).
+  (*
+  destruct (n0, b0).
+  rewrite H1; auto. simpl. destruct b; simpl; rewrite <- H; auto.
+  admit.
+  admit. *)
+Admitted.
+
